stuck on thm I, working on thm II

work_param.v
@@ -3,7 +3,9 @@ Require Import Psatz.
 Require Export Setoid Morphisms.
 Set Implicit Arguments.
 
-Class B_param (B : Type) (X : Type) := {
+Section B.
+
+Class B_param (B : Type) := {
   is_true : B -> Prop; (* need this to define everything *)
   BFalse : B; (* need this to define bottom in a CL *)
   BTrue : B; (* idem *)
@@ -15,11 +17,28 @@ Class B_param (B : Type) (X : Type) := {
   BOr_spec : forall b1 b2, is_true b1 \/ is_true b2 <-> is_true (BOr b1 b2);
   BImpl : B -> B -> B;
   BImpl_spec : forall b1 b2, (is_true b1 -> is_true b2) <-> (is_true (BImpl b1 b2));
-  BForall : (X -> B) -> B;
+  }.
+
+Definition BEq `{B_param} PB1 PB2 := BAnd (BImpl PB1 PB2) (BImpl PB2 PB1).
+Lemma BEq_spec `{B_param} : forall b1 b2, (is_true b1 <-> is_true b2) <-> is_true (BEq b1 b2).
+Proof. intros b1 b2. setoid_rewrite <- BAnd_spec. setoid_rewrite <- BImpl_spec. tauto. Qed.
+
+#[global] Instance trans_Impl `{B_param} : Transitive (fun b1 b2 => is_true (BImpl b1 b2)).
+Proof. intros b1 b2 b3. setoid_rewrite <- BImpl_spec. tauto. Qed.
+#[global] Instance refl_Impl `{B_param} : Reflexive (fun b1 b2 => is_true (BImpl b1 b2)).
+Proof. intro b1. setoid_rewrite <- BImpl_spec. tauto. Qed.
+
+Class B_param_plus (B : Type) (X : Type) `(B_param B) := {
+  BForall : (X -> B) -> B;(*Needed for Inf, for comparison of monotonous functions, and for set equality.*)
   BForall_spec : forall (P : X -> B), (forall x, is_true (P x)) <-> is_true (BForall P);
-  BExists : (X -> B) -> B;
+  BExists : (X -> B) -> B; (*Needed for Images of functions and monotonous complete lattice*)
   BExists_spec : forall (P : X -> B), (exists x, is_true (P x)) <-> is_true (BExists P);
+  BExists_set : ((X -> B) -> B) -> B; (*needed for the Complete Lattice of parts/subsets*)
+  BExists_set_spec : forall (P : (X -> B) -> B), (exists S, is_true (P S)) <-> is_true (BExists_set P);
   
+  
+  BExists_nat : (nat -> B) -> B;
+  BExists_nat_spec : forall (P : nat -> B), (exists n, is_true (P n)) <-> is_true (BExists_nat P);
   (*
   BForall_g (A:Type) : (A -> B) -> (A -> B) -> B; (*here I is to select only a subset of A according to some condition B
     and bfun is the property that need to be true for all element in that subset *)
@@ -44,7 +63,26 @@ Class B_param (B : Type) (X : Type) := {
   B_impl_trans : forall x y z, is_true (B_impl x y) -> is_true (B_impl y z) -> is_true (B_impl x z);*)
   }.
 
-Class B_PO (X: Type) (B : Type) (Bp : B_param B X) := {
+End B.
+
+Section CPO_CL.
+
+Context {X : Type} {B} {Bp : B_param B}.  (*{Bpp : B_param_plus X Bp}.*)
+
+Notation set := (X -> B).
+Notation rel := (X -> X -> B).
+(*
+Definition weq_in_prop `(weq : rel) (x y : X) := is_true (weq x y).
+Definition leq_in_prop `(leq : rel) (x y : X) := is_true (leq x y).
+Definition Directed `(leq_in_prop : X -> X -> Prop) (D : set) : Prop :=
+  forall x y, is_true (D x) -> is_true (D y) -> exists z, is_true (D z) /\ leq_in_prop x z /\ leq_in_prop y z.
+Definition directed_set `(leq_in_prop : X -> X -> Prop) := 
+  {Dbody : set | Directed leq_in_prop Dbody}.
+Definition Dbody `(leq_in_prop : X -> X -> Prop) (D : directed_set leq_in_prop) : set := 
+  proj1_sig D.
+  *)
+
+Class B_PO := {
     weq: X -> X -> B;
     leq: X -> X -> B;
     weq_in_prop x y := is_true (weq x y);
@@ -55,17 +93,32 @@ Class B_PO (X: Type) (B : Type) (Bp : B_param B X) := {
     weq_spec: forall x y, weq_in_prop x y <-> leq_in_prop x y /\ leq_in_prop y x;
   }.
 
+
 (*
 Definition weq_in_prop {X} {B} {Bp : B_param B} {L' : B_PO X Bp} (x y : X) := is_true (B := B) (weq x y).
 Definition leq_in_prop {X} {B} {Bp : B_param B} {L' : B_PO X Bp} (x y : X) := is_true (B := B) (leq x y).
 *)
 
-(* Definition of Lattice as a particular (stronger) CPO. *)
-Class B_CL (X : Type) (B : Type) (Bp : B_param B X) `(L' : B_PO X) := {
-    sup: (X -> B) -> X;
-    (*sup_spec0 : forall Y y, is_true (Y y) -> is_true (leq y (sup Y));*)
-    sup_spec: forall Y z, leq_in_prop (sup Y) z <-> (forall y, is_true (Y y) -> leq_in_prop y z);
+Definition Directed (D : set) `(leq_in_prop : X -> X -> Prop) : Prop := 
+  forall x y, is_true (D x) -> is_true (D y) -> exists z, is_true (D z) /\ leq_in_prop x z /\ leq_in_prop y z.
+Definition directed_set `(leq_in_prop : X -> X -> Prop) := {Dbody : set | Directed Dbody leq_in_prop}.
+Definition Dbody `(leq_in_prop : X -> X -> Prop) (D : directed_set leq_in_prop) : set := proj1_sig D.
+Coercion Dbody : directed_set >-> Funclass.
+
+Class B_CPO `(P' : B_PO) := {
+    sup: directed_set leq_in_prop -> X;
+    sup_spec: forall D z, (leq_in_prop (sup D) z <-> forall (y:X), is_true ((Dbody D) y) -> leq_in_prop y z);
   }.
+
+(* Definition of Lattice as a particular (stronger) CPO. *)
+Class B_CL `(L' : B_PO) := {
+    Sup: (X -> B) -> X;
+    (*sup_spec0 : forall Y y, is_true (Y y) -> is_true (leq y (sup Y));*)
+    Sup_spec: forall Y z, leq_in_prop (Sup Y) z <-> (forall y, is_true (Y y) -> leq_in_prop y z);
+  }.
+  (* Convention : capital letters for CL from now on. *)
+
+End CPO_CL.
 
 Declare Scope B_PO.
 Open Scope B_PO.
@@ -74,130 +127,10 @@ Infix "<=" := leq_in_prop (at level 70): B_PO.
 #[global] Hint Extern 0 => reflexivity: core.
 
 
-Section Partial_order.
-
-  Context {X} `{P' : B_PO X}.
-(*
-  #[global] Instance Preorder_leq : PreOrder leq_in_prop.
-  Proof.
-    constructor.
-    intro x. apply leq_refl.
-    intros x y z. apply leq_trans.
-  Qed.
-*)
-  #[global] Instance Equivalence_weq: Equivalence weq_in_prop.
-  Proof.
-    constructor.
-    intro x. now apply weq_spec.
-    intros x y. rewrite 2weq_spec. tauto.
-    intros x y z. rewrite 3weq_spec. split; transitivity y; tauto.
-  Qed.
-
-  #[global] Instance PartialOrder_weq_leq: PartialOrder weq_in_prop leq_in_prop.
-  Proof.
-    intros x y. cbn. now rewrite weq_spec.
-  Qed.
-
-End Partial_order.
-
-
-
-Section sup.
-
-  Context {X} {B} {Bp : B_param B X} {P' : B_PO Bp} {L : B_CL Bp P'}.
-
-  Lemma leq_xsup (Y: X -> B) y : is_true (Y y) -> y <= sup Y.
-  Proof. intro H. now apply (sup_spec Y). Qed.
-
-  Definition bot := sup (fun _ => BFalse).
-  
-  Lemma bot_spec: forall x, bot <= x.
-  Proof. intro. apply sup_spec. intros y Hy. contradict Hy. apply BFalse_spec. Qed.
-
-  Definition top := sup (fun _ => BTrue).
-
-  Lemma top_spec: forall x, x <= top.
-  Proof. intro. apply leq_xsup. apply BTrue_spec. Qed.
-
-  (** Inf *)
-
-  Definition inf (Y : X -> B) := sup (fun z => BForall (fun y => BImpl (Y y) (leq z y))).
-  Lemma inf_spec : forall Y z, z <= inf Y <-> (forall y, is_true (Y y) -> z <= y).
-  Proof.
-    intros. split.
-    intros H y Yy. rewrite H. apply sup_spec. intros y0 H0.
-    rewrite <- BForall_spec in H0. setoid_rewrite <- BImpl_spec in H0. now apply (H0 y).
-    intro. apply leq_xsup. apply -> BForall_spec. intro y. apply -> BImpl_spec. intro. now apply H.
-  Qed.
-
-  Lemma leq_xinf (D: X -> B) y:  is_true (D y) -> inf D <= y.
-  Proof. intro H. now apply inf_spec with D. Qed.
-
-End sup.
-
-#[global] Hint Resolve bot_spec: core.
-
-
-
-Section function.
-
-  Context {X} {B} {Bp : B_param B X} {P' : B_PO Bp}. 
-
-  Record mon := { body:> X -> X; Hbody: Proper (leq_in_prop ==> leq_in_prop) body }.
-
-  #[global] Instance Hbody' (F:mon) : Proper (weq_in_prop ==> weq_in_prop) F.
-  Proof. intros x y Hxy. apply weq_spec. split; apply Hbody; now apply weq_spec in Hxy. Qed.
-
-End function.
-
-
-
-(* Knaster-Tarski Theorem on Lattices *)
-
-Section lattice_results.
-  Context {X} {B} {Bp : B_param B X} {P' : B_PO Bp} {L : B_CL Bp P'}.
-  Variable b: mon.
-
-  Definition gfp := sup (fun x => leq x (b x)).
-  Definition lfp := inf (fun x => leq (b x) x).
-
-  Proposition leq_gfp: forall y, y <= b y -> y <= gfp.
-  Proof. apply leq_xsup. Qed.
-  Proposition geq_lfp: forall y, b y <= y -> lfp <= y.
-  Proof. apply leq_xinf. Qed.
-
-  Lemma gfp_pfp: gfp <= b gfp.
-  Proof.
-    unfold gfp. apply sup_spec. intros y H. rewrite H. apply Hbody.
-    apply leq_xsup. apply H.
-  Qed.
-  Lemma lfp_pfp: b lfp <= lfp.
-  Proof.
-    unfold lfp. apply inf_spec. intros y H. rewrite <- H. apply Hbody.
-    apply leq_xinf. apply H.
-  Qed.
-
-  Lemma gfp_fp: gfp == b gfp.
-  Proof.
-    rewrite weq_spec. split.
-    + apply gfp_pfp.
-    + apply leq_xsup. apply Hbody. apply gfp_pfp.
-  Qed.
-  Lemma lfp_fp: lfp == b lfp.
-  Proof.
-    rewrite weq_spec. split.
-    + apply leq_xinf. apply Hbody. apply lfp_pfp.
-    + apply lfp_pfp.
-  Qed.
-
-End lattice_results.
-
-
 
 Section Concrete_Examples.
-
+(*
 Require Import Bool.
-
 
 Program Instance Prop_B (X: Type): B_param Prop X :=
   {|
@@ -243,7 +176,382 @@ Program Instance bool_B : B_param bool A :=
     exists x. split. apply HList. now apply Is_true_eq_true.
     apply Is_true_eq_true in H. apply List.existsb_exists in H. destruct H as [x Hx]. exists x.
     apply Is_true_eq_left. apply Hx. Qed.
-
+*)
 End Concrete_Examples.
+
+
+Section Partial_order.
+
+  Context {X} `{P' : B_PO X}.
+(*
+  #[global] Instance Preorder_leq : PreOrder leq_in_prop.
+  Proof.
+    constructor.
+    intro x. apply leq_refl.
+    intros x y z. apply leq_trans.
+  Qed.
+*)
+  #[global] Instance Equivalence_weq: Equivalence weq_in_prop.
+  Proof.
+    constructor.
+    intro x. now apply weq_spec.
+    intros x y. rewrite 2weq_spec. tauto.
+    intros x y z. rewrite 3weq_spec. split; transitivity y; tauto.
+  Qed.
+
+  #[global] Instance PartialOrder_weq_leq: PartialOrder weq_in_prop leq_in_prop.
+  Proof.
+    intros x y. cbn. now rewrite weq_spec.
+  Qed.
+  
+  Record mon := { body:> X -> X; Hbody: Proper (leq_in_prop ==> leq_in_prop) body }.
+
+End Partial_order.
+
+
+
+Section sup.
+
+  Context {X} {B} {Bp : B_param B} {P' : B_PO (X := X)} {P : B_CPO P'} {L : B_CL P'}.
+  Context {Bpp : B_param_plus X Bp}.
+
+  Lemma leq_xsup (D: directed_set leq_in_prop) (y : X) : is_true (D y) -> y <= sup D.
+  Proof. intro H. now apply (sup_spec D). Qed.
+  Lemma leq_xSup (Y: X -> B) (y : X) : is_true (Y y) -> y <= Sup Y.
+  Proof. intro H. now apply (Sup_spec Y). Qed.
+
+  Program Definition empty : directed_set leq_in_prop :=
+    exist _ (fun _ => BFalse) _.
+  Next Obligation. unfold Directed. intros. contradict H. apply BFalse_spec. Defined.
+
+  Definition bot := sup empty.
+  Definition Bot := Sup (fun _ => BFalse). (* CompleteLattice Bot *)
+  (* Rmk : insteaf of working with notions from CPO and CL alike, we could just turn a CL into a CPO,
+  but for basic notion like this, it might be better to have both *)
+  
+  Lemma bot_spec : forall x, bot <= x.
+  Proof. intro. apply sup_spec. intros y Hy. contradict Hy. apply BFalse_spec. Qed.
+  Lemma Bot_spec: forall x, Bot <= x.
+  Proof. intro. apply Sup_spec. intros y Hy. contradict Hy. apply BFalse_spec. Qed.
+
+  Definition Top := Sup (fun _ => BTrue).
+
+  Lemma Top_spec: forall x, x <= Top.
+  Proof. intro. apply leq_xSup. apply BTrue_spec. Qed.
+
+  (** Inf *)
+
+  Definition Inf (Y : X -> B) := Sup (fun z => BForall (fun y => BImpl (Y y) (leq z y))).
+  Lemma Inf_spec : forall Y z, z <= Inf Y <-> (forall y, is_true (Y y) -> z <= y).
+  Proof.
+    intros. split.
+    intros H y Yy. rewrite H. apply Sup_spec. intros y0 H0.
+    rewrite <- BForall_spec in H0. setoid_rewrite <- BImpl_spec in H0. now apply (H0 y).
+    intro. apply leq_xSup. apply -> BForall_spec. intro y. apply -> BImpl_spec. intro. now apply H.
+  Qed.
+
+  Lemma leq_xInf (D: X -> B) y:  is_true (D y) -> Inf D <= y.
+  Proof. intro H. now apply Inf_spec with D. Qed.
+
+End sup.
+
+#[global] Hint Resolve bot_spec: core.
+#[global] Hint Resolve Bot_spec: core.
+
+
+
+(* Knaster-Tarski Theorem on Lattices *)
+
+Section lattice_results.
+  Context {X} {B} {Bp : B_param B} {P' : B_PO (X := X)} {L : B_CL P'}.
+  Context {Bpp : B_param_plus X Bp}.
+  Variable b: mon.
+
+  Definition gfp := Sup (fun x => leq x (b x)).
+  Definition lfp := Inf (fun x => leq (b x) x).
+
+  Proposition leq_gfp: forall y, y <= b y -> y <= gfp.
+  Proof. apply leq_xSup. Qed.
+  Proposition geq_lfp: forall y, b y <= y -> lfp <= y.
+  Proof. apply leq_xInf. Qed.
+
+  Lemma gfp_pfp: gfp <= b gfp.
+  Proof.
+    unfold gfp. apply Sup_spec. intros y H. rewrite H. apply Hbody.
+    apply leq_xSup. apply H.
+  Qed.
+  Lemma lfp_pfp: b lfp <= lfp.
+  Proof.
+    unfold lfp. apply Inf_spec. intros y H. rewrite <- H. apply Hbody.
+    apply leq_xInf. apply H.
+  Qed.
+
+  Lemma gfp_fp: gfp == b gfp.
+  Proof.
+    rewrite weq_spec. split.
+    + apply gfp_pfp.
+    + apply leq_xSup. apply Hbody. apply gfp_pfp.
+  Qed.
+  Lemma lfp_fp: lfp == b lfp.
+  Proof.
+    rewrite weq_spec. split.
+    + apply leq_xInf. apply Hbody. apply lfp_pfp.
+    + apply lfp_pfp.
+  Qed.
+
+End lattice_results.
+
+
+
+Section function.
+
+  Context {X} {B} {Bp : B_param B} {P' : B_PO (X := X)} {P : B_CPO P'}.
+  Context {Bpp : B_param_plus X Bp}.
+
+  Definition Fix F x := F x == x.
+  Definition Post F x := x <= F x.
+  Definition Pre F x := F x <= x.
+
+  Lemma fix_is_post F : forall x, Fix F x -> Post F x.
+  Proof. intros. apply weq_spec in H. apply H. Qed.
+  Lemma fix_is_pre F : forall x, Fix F x -> Pre F x.
+  Proof. intros. apply weq_spec in H. apply H. Qed.
+
+  #[global] Instance Hbody' (F:mon) : Proper (weq_in_prop ==> weq_in_prop) F.
+  Proof. intros x y Hxy. apply weq_spec. split; apply Hbody; now apply weq_spec in Hxy. Qed.
+
+  Definition Image f (S : X -> B) y := (BExists (fun x => BAnd (S x) (weq y (f x)))).
+
+  Definition Continuous f :=
+    forall (D : X -> B) (H : Directed D leq_in_prop),
+      {dir_im : Directed (Image f D) leq_in_prop &
+                f (sup (exist _ D H )) == sup (exist _ (Image f D) dir_im)}.
+
+  Lemma mon_preserves_directedness_and_sup (F:mon) :
+    forall (D : X -> B) (H : Directed D leq_in_prop),
+      {dir_im : Directed (Image F D) leq_in_prop &
+                  sup (exist _ (Image F D) dir_im) <= F (sup (exist _ D H ))}.
+  Proof.
+    intros. assert (Directed (Image F D) leq_in_prop) as DD.
+    + unfold Directed. intros y1 y2 Hfy1 Hfy2. apply BExists_spec in Hfy1, Hfy2. 
+      destruct Hfy1 as [x1 Hx1]. destruct Hfy2 as [x2 Hx2].
+      apply BAnd_spec in Hx1, Hx2. destruct Hx1 as [Dx1 Hx1]. destruct Hx2 as [Dx2 Hx2].
+      destruct (H x1 x2) as [x Hx]; try assumption.
+      exists (F x). repeat split. apply BExists_spec. exists x. apply BAnd_spec. split.
+      apply Hx. fold (weq_in_prop (F x) (F x)). reflexivity. rewrite Hx1.
+      now apply Hbody. rewrite Hx2. now apply Hbody.
+    + exists DD. apply sup_spec; cbn. intros y Hy.
+      apply BExists_spec in Hy. destruct Hy as [x Hx]. apply BAnd_spec in Hx. destruct Hx as [Dx Hx].
+      rewrite Hx. apply Hbody. now apply leq_xsup.
+  Qed.
+
+(* Iterations of a function *)
+
+
+  Definition foo (x:X) (f : {x = bot} + {x <> bot}) : Prop := match f with | left _ => True | right _ => False end.
+
+(*
+  Fixpoint iteres F (y : X) (is_bot_y : {y = bot} + {y <> bot}) : B := match is_bot_y with
+  | left _ => BTrue
+  | right _ => BExists (fun x => BAnd (weq y (F x)) (iteres F x))
+  end.
+  
+  | iteres_0 : (iteres F bot)
+  | iteres_S : forall x, (iteres F x) -> (iteres F (F x)).
+
+*)
+  Fixpoint itere F n x0 : X :=
+    match n with
+    | 0 => x0
+    | S m => F (itere F m x0)
+    end. (*Indexed by n for simplicity on comparison properties.*)
+
+  Lemma itere_monotony (F:mon) : forall n, Proper (leq_in_prop ==> leq_in_prop) (itere F n).
+  Proof. intros n x y H. induction n. now cbn. cbn. now apply Hbody. Qed.
+
+  Lemma chain_itere (F:mon) : forall (n : nat), itere F n bot <= itere F (S n) bot.
+  Proof. intro n. induction n. now cbn. cbn. now apply Hbody. Qed.
+
+  Lemma chain_increase (F:mon) : forall (m n : nat), le n m -> itere F n bot <= itere F m bot.
+  Proof.
+    intros m n H. induction m. now inversion H.
+    inversion H. easy.
+    rewrite <- chain_itere. now apply IHm.
+  Qed.
+
+  Lemma itere_preserves_fix (F:mon) : forall β n, Fix F β -> (itere F n β) == β.
+  Proof.
+    intros. induction n. now cbn. cbn. unfold Fix in H. rewrite <- H at 2.
+    now apply Hbody'.
+  Qed.
+
+  Definition iteres F x : B := BExists_nat (fun n => weq x (itere F n bot)).
+
+(* TODO !
+  Definition iteres F : X -> B :=
+  | from_bot : forall n, iteres F (itere F n bot).
+
+  Lemma iteres_directed (F:mon): Directed (iteres F).
+  Proof.
+    unfold Directed. intros. destruct H. destruct H0.
+    destruct le_ge_dec with n n0.
+    + exists (itere F n0 bot). repeat split. now apply chain_increase. reflexivity.
+    + exists (itere F n bot). repeat split. reflexivity. now apply chain_increase.
+  Qed.
+
+  Variant iteres_from_1 F : X -> Prop :=
+  | from_bot_from_1 : forall n, le 1 n -> iteres_from_1 F (itere F n bot).
+
+  Lemma iteres_from_1_directed (F:mon): Directed leq (iteres_from_1 F).
+  Proof.
+    unfold Directed. intros. destruct H. destruct H0.
+    destruct le_ge_dec with n n0.
+    + exists (itere F n0 bot). repeat split. assumption. now apply chain_increase. reflexivity.
+    + exists (itere F n bot). repeat split. assumption. reflexivity. now apply chain_increase.
+  Qed.
+
+  Lemma image_of_iteres F : set_eq (Image F (iteres F)) (iteres_from_1 F).
+  Proof.
+    intro. split; intro; inversion H. inversion H0.
+    + assert (iteres_from_1 F (itere F (S n) bot)). apply from_bot_from_1. lia.
+      apply H3.
+    + induction n. contradict H0. lia.
+      cbn. apply from_image. apply from_bot.
+  Qed.
+
+  Lemma from_1_included F : included (iteres_from_1 F) (iteres F).
+  Proof. intros x H. inversion H. apply from_bot. Qed.
+*)
+End function.
+
+
+
+(** * Sets general properties *)
+
+Section Sets.
+
+  Context {X} {B} {Bp : B_param B} {P' : B_PO (X := X)}.
+  Context {Bpp : B_param_plus X Bp}.
+
+  Definition set_eq (f g : X -> B) :=  (BForall (B_param_plus := Bpp)) (fun z => (BEq (f z) (g z))). (*equality of sets*)
+
+  Definition included (S T: X -> B) := BForall (B_param_plus := Bpp) (fun x => (BImpl (S x) (T x))).
+  
+  Definition included_prop (S T : X -> B) := is_true (included S T).
+  
+End Sets.
+Infix "⊆" := included_prop (at level 70).
+
+
+
+
+Section Particular_CPOs.
+
+  Context {X} {B} {Bp : B_param B} {P' : B_PO (X := X)} {P : B_CPO P'}.
+  Context {Bpp : B_param_plus X Bp} {Bpp_mon : B_param_plus mon Bp}.
+
+ Program Instance B_PO_mon : @B_PO mon B Bp :=
+    {|
+      weq f g := BForall (fun (x:X) => weq (f x) (g x));
+      leq f g := BForall (fun (x:X) => leq (f x) (g x));
+    |}.
+  Next Obligation.
+  apply Build_PreOrder.
+    + intro x. apply BForall_spec. intro. fold (leq_in_prop (x x0) (x x0)). reflexivity.
+    + intros f g h Hfg Hgh. apply BForall_spec. intro x. fold (leq_in_prop (f x) (h x)).
+      rewrite <- BForall_spec in Hfg, Hgh.
+      transitivity (g x). apply Hfg. apply Hgh.
+  Qed.
+  Next Obligation.
+    setoid_rewrite <- BForall_spec.
+    split; intros.
+    + split; intro a; apply weq_spec. symmetry; apply H. apply H.
+    + apply weq_spec. split; apply H.
+  Qed.
+
+  Program Instance B_CPO_mon : B_CPO B_PO_mon :=
+    {|
+      sup (F : @directed_set mon B Bp leq_in_prop) := {| body x := sup (fun y => BExists (*B mon Bp Bpp_mon*) (fun f => BAnd (F f) (weq y (f x)))) |};
+    |}.
+  Next Obligation.
+    unfold Directed. setoid_rewrite <- BExists_spec.
+    intros. destruct F as [SF D]; cbn in *.
+    destruct H as [fx Hfx]. destruct H0 as [fy Hfy]. rewrite <- BAnd_spec in Hfx, Hfy.
+    destruct Hfx as [Hfx Eqfx]. destruct Hfy as [Hfy Eqfy].
+    destruct (D fx fy) as [f [Hf1S [Hff1 Hff2]]]; try assumption.
+    exists (f x). unfold leq_in_prop in Hff1, Hff2. cbn in *. rewrite <- BForall_spec in Hff1, Hff2.
+    repeat split. exists f. apply BAnd_spec. split. 
+    assumption. fold (weq_in_prop (f x) (f x)). reflexivity.
+                                 + rewrite Eqfx. apply (Hff1 x).
+                                 + rewrite Eqfy. apply (Hff2 x).
+  Qed.
+  Next Obligation.
+    destruct F as [SF D]; cbn in *.
+    intros x y H. apply sup_spec; cbn. intros.
+    rewrite <- BExists_spec in H0. setoid_rewrite <- BAnd_spec in H0.
+    destruct H0 as [f [Hfx0 Eqyx]].
+    transitivity (f y). rewrite Eqyx. now apply Hbody.
+    apply leq_xsup. cbn. apply BExists_spec. exists f. apply BAnd_spec.
+    split. assumption. fold (weq_in_prop (f y) (f y)). reflexivity.
+  Qed.
+  Next Obligation.
+    destruct D as [SF D]; cbn in *. split.
+    + intros H f Df. unfold leq_in_prop in *. cbn in *. rewrite <- BForall_spec in *. intro x.
+      fold (leq_in_prop (f x) (z x)). rewrite <- H.
+      eapply sup_spec. reflexivity. cbn. apply BExists_spec. exists f. apply BAnd_spec. split. assumption.
+      now fold (weq_in_prop (f x) (f x)).
+    + intro H. unfold leq_in_prop. cbn. apply BForall_spec. intro x. apply sup_spec. cbn. intros y Hy.
+      rewrite <- BExists_spec in Hy. destruct Hy as [f Hf]. apply BAnd_spec in Hf. destruct Hf as [Hf Eqyfx].
+      rewrite Eqyfx. unfold leq_in_prop in H. cbn in H. setoid_rewrite <- BForall_spec in H. now apply (H f).
+  Qed.
+
+  Program Instance B_PO_parts: @B_PO (X -> B) B Bp :=
+    {|
+      weq := set_eq;
+      leq := included;
+    |}.
+  Next Obligation.
+    apply Build_PreOrder.
+    + intro Y. apply BForall_spec. intro x. apply refl_Impl.
+    + intros S T U. setoid_rewrite <- BForall_spec. intros. now apply (trans_Impl (S x)) with (T x).
+  Qed.
+  Next Obligation.
+    setoid_rewrite <- BForall_spec. setoid_rewrite <- BEq_spec. setoid_rewrite <- BImpl_spec.
+    intuition; now apply H.
+  Qed.
+
+  Program Instance B_CPO_parts: B_CPO B_PO_parts :=
+    {|
+      sup A := (fun x => BExists_set (fun Y => BAnd (A Y) (Y x)));
+    |}.
+  Next Obligation.
+    unfold leq_in_prop; cbn. split; intros. 
+    + apply BForall_spec. intro x. apply BImpl_spec. intro Hx.
+      setoid_rewrite <- BForall_spec in H. setoid_rewrite <- BImpl_spec in H. 
+      setoid_rewrite <- BExists_set_spec in H. apply (H x). exists y. apply BAnd_spec. now split.
+    + apply BForall_spec. intro x. apply BImpl_spec. intro PDx. 
+      rewrite <- BExists_set_spec in PDx. setoid_rewrite <- BAnd_spec in PDx. destruct PDx as [S [Ds Sx]].
+      specialize H with S. apply H in Ds. setoid_rewrite <- BForall_spec in Ds. setoid_rewrite <- BImpl_spec in Ds.
+      now apply Ds.
+  Qed.
+
+  Program Instance Lattice_parts : B_CL (B_PO_parts) :=
+    {|
+      Sup A := (fun x => BExists_set (fun Y => BAnd (A Y) (Y x)));
+    |}.
+  Next Obligation.
+   unfold leq_in_prop; cbn. split; intros. 
+    + apply BForall_spec. intro x. apply BImpl_spec. intro Hx.
+      setoid_rewrite <- BForall_spec in H. setoid_rewrite <- BImpl_spec in H. 
+      setoid_rewrite <- BExists_set_spec in H. apply (H x). exists y. apply BAnd_spec. now split.
+    + apply BForall_spec. intro x. apply BImpl_spec. intro PDx. 
+      rewrite <- BExists_set_spec in PDx. setoid_rewrite <- BAnd_spec in PDx. destruct PDx as [S [Ds Sx]].
+      specialize H with S. apply H in Ds. setoid_rewrite <- BForall_spec in Ds. setoid_rewrite <- BImpl_spec in Ds.
+      now apply Ds.
+   Qed.
+
+End Particular_CPOs.
+
+
 
 
